Diff/UcoPreservation.v
@@ -1,0 +1,84 @@
+From mathcomp Require Import all_ssreflect. 
+
+Set Implicit Arguments.
+Unset Printing Implicit Defensive.
+
+Require Import ClassicalExtras.
+Require Import MyNotation.
+Require Import Setoid.
+Require Import FunctionalExtensionality.
+
+Require Import Galois.
+Require Import LanguageModel.
+Require Import TraceModel.
+Require Import Properties.
+Require Import ChainModel.
+Require Import NonRobustDef.
+
+Section Closure_Operators_Preservation.
+
+ (* Every time we can express a Class Ξ via an upper closed operator ξ
+     we have that γΞP is equivalent to (ξ ∘ τ)TP. 
+    
+     for instance we can express the class of Safety properties using 
+     the uco Cl. *)
+
+
+   Variable Source Target: Language.
+  Variable compilation_chain : CompilationChain Source Target.
+  
+  Variable Σ__S Σ__T States__S States__T : Set.
+  Variable E__S : Events Σ__S.
+  Variable E__T : Events Σ__T.
+  Variable S__S : EndState States__S.
+  Variable S__T : EndState States__T.
+
+  Local Definition trace__S := trace Σ__S States__S.
+  Local Definition trace__T := trace Σ__T States__T.
+  Local Definition prop__S := prop Σ__S States__S.
+  Local Definition prop__T := prop Σ__T States__T.
+  
+  Variable sem__S : prg Source -> trace__S -> Prop.
+  Variable non_empty_sem__S : forall W, exists s, sem__S W s.   
+
+  Variable sem__T : prg Target -> trace__T -> Prop.
+  Variable non_empty_sem__T : forall W, exists t, sem__T W t.   
+  
+  Local Definition prg__S := prg Source.
+  Local Definition prg__T := prg Target.
+
+  Local Definition sat__S := sat Source sem__S.
+  Local Definition sat__T := sat Target sem__T.
+  
+  Local Definition cmp := compile_whole Source Target compilation_chain.
+
+  Local Notation "W ↓" := (cmp W) (at level 50).
+ 
+   
+  (*CA: issue! prop__T : Type but not prop__T : Set! *)
+  Variable cl_operator : (Uco prop__T).  
+
+  
+  
+  Lemma uco_adjuncts_rp' (f: Uco ) :
+    Adjunction_law τ σ -> 
+    ( (forall W (π__T : prop__T),  σP W ((uco f) π__T)) <->                    
+      (τTP ((uco f) ∘ τ))).
+  Proof. 
+    rewrite Galois_equiv. move => [mono_γ [mono_τ [G1 G2]]].
+    split => H_rp P π rsat_src.  
+    + have H: rsat P (γ ((uco f) (τ π))).
+      { apply: rsat_upper_closed. exact: rsat_src.
+        apply: (@prop_subset_trans source π (γ (τ π))). by apply: G1. 
+        apply: mono_γ. exact: (ext f). }  
+      move: (H_rp P (((uco f) (τ π)))). firstorder. 
+    + have H: rsat (P ↓) ((uco f) π).
+      { move: (H_rp P _ rsat_src) => H.
+        apply: rsat_upper_closed. exact: H.
+        apply: (@prop_subset_trans target _ ((uco f) (uco f π)) _).
+        apply: mono. by apply: G2.
+          by rewrite (idmp f). }
+      exact: H. 
+  Qed.
+
+End Closure_Operators_Preservation. 
